wip: Serializability proof for the prototype

src/Prototype/Language.v
@@ -50,20 +50,29 @@ Section Language.
     Definition ObjectStates :=
       Map IdxT { StateT : Type & ObjectState StateT }.
 
-    Definition InMsgs := Map IdxT (list Msg).
+    Definition InMsgs := Map IdxT (* from *) (list Msg).
 
-    Definition ObjectInMsgs := Map IdxT InMsgs.
+    Definition ObjectInMsgs := Map (IdxT * bool) (* (to, is_req) *) InMsgs.
 
     Definition idx_add {A} (k: IdxT) (v: A) m :=
       add eq_nat_dec k v m.
 
+    Definition idx_bool_dec: forall (k1 k2: IdxT * bool), {k1 = k2} + {k1 <> k2}.
+    Proof.
+      decide equality.
+      - apply Bool.bool_dec.
+      - apply eq_nat_dec.
+    Defined.
+    Definition idx_bool_add {A} (k: IdxT * bool) (v: A) m :=
+      add idx_bool_dec k v m.
+
     Fixpoint step_rule {StateT} (rules: list (RuleT StateT))
              (imsg: IMsg) (st: StateT) :=
       match rules with
-      | nil => (nil, None, st)
+      | nil => None
       | r :: rules' =>
         match r imsg st with 
-        | Some mst => mst
+        | Some mst => Some mst
         | None => step_rule rules' imsg st
         end
       end.
@@ -74,7 +83,7 @@ Section Language.
       ObjectState StateT -> InMsgs -> Prop :=
     | StepObjInt: forall os imsgs fidx fmsg fmsgs imsgs_to emsgs_to pos,
         step_rule (obj_rules (os_obj os)) (fidx, fmsg) (os_state os) =
-        (imsgs_to, emsgs_to, pos) ->
+        Some (imsgs_to, emsgs_to, pos) ->
         find fidx imsgs = Some (fmsg :: fmsgs) ->
         step_obj os imsgs
                  imsgs_to None emsgs_to
@@ -83,7 +92,7 @@ Section Language.
                  (idx_add fidx fmsgs imsgs)
     | StepObjExt: forall os imsgs emsg_in imsgs_to emsgs_to pos,
         step_rule (obj_rules (os_obj os)) emsg_in (os_state os) =
-        (imsgs_to, emsgs_to, pos) ->
+        Some (imsgs_to, emsgs_to, pos) ->
         step_obj os imsgs
                  imsgs_to (Some emsg_in) emsgs_to
                  {| os_obj := os_obj os;
@@ -95,33 +104,34 @@ Section Language.
       match to with
       | nil => msgs
       | (toIdx, msg) :: to' =>
-        match msgs toIdx with
+        match find (toIdx, msg_is_req msg) msgs with
         | Some toMsgs =>
           let added := match toMsgs from with
                        | Some fromMsgs => fromMsgs ++ (msg :: nil)
                        | None => msg :: nil
                        end in
-          idx_add toIdx (idx_add from added toMsgs) msgs
+          idx_bool_add (toIdx, msg_is_req msg) (idx_add from added toMsgs) msgs
         | None =>
-          idx_add toIdx (idx_add from (msg :: nil) (@empty _ _)) msgs
+          idx_bool_add (toIdx, msg_is_req msg) (idx_add from (msg :: nil) (@empty _ _)) msgs
         end
       end.
 
     Inductive step : ObjectStates -> ObjectInMsgs ->
                      option IMsg (* external in *) -> option IMsg (* external out *) ->
                      ObjectStates -> ObjectInMsgs -> Prop :=
-    | Step: forall oss idx {StateT} (os: ObjectState StateT)
+    | Step: forall oss idx is_req {StateT} (os: ObjectState StateT)
                    oims imsgs imsgs_to emsg_in emsg_out pos pimsgs,
         find idx oss = Some (existT _ _ os) ->
-        find idx oims = Some imsgs -> 
+        find (idx, is_req) oims = Some imsgs -> 
         step_obj os imsgs imsgs_to emsg_in emsg_out pos pimsgs ->
         step oss oims emsg_in emsg_out
              (idx_add idx (existT _ _ pos) oss)
-             (distr_msgs idx imsgs_to (idx_add idx pimsgs oims)).
+             (distr_msgs idx imsgs_to (idx_bool_add (idx, is_req) pimsgs oims)).
 
+    (* NOTE: the oldest is the head *)
     Definition addHistory (om: option IMsg) (hst: list IMsg) :=
       match om with
-      | Some m => m :: hst
+      | Some m => hst ++ (m :: nil)
       | None => hst
       end.
     Infix "<::" := addHistory (at level 30, right associativity).
@@ -152,18 +162,28 @@ Section Language.
     Definition HistoryOf (obs: Objects) (hst: list IMsg) :=
       exists oss oims, steps (getObjectStatesInit obs) (@empty _ _) hst oss oims.
 
-    Fixpoint serial' (hst: list IMsg) (oi: option IdxT) :=
+    (** Now some notions borrowed from linearlizability and serializability.
+     * Definitions need to be much more robust for the real language design.
+     * It's for now a bit informal.
+     *)
+
+    (* A maximum subsequence of H consisting only of requests and matching responses. *)
+    Definition complete (hst: list IMsg): list IMsg. Admitted.
+
+    Definition Complete (hst: list IMsg) := hst = complete hst.
+
+    Fixpoint Serial' (hst: list IMsg) (oi: option IdxT) :=
       match hst with
       | nil => True
       | (idx, msg) :: hst' =>
         match oi with
         | Some i => idx = i /\ msg_is_req msg = false /\
-                    serial' hst' None
-        | None => msg_is_req msg = true /\ serial' hst' (Some idx)
+                    Serial' hst' None
+        | None => msg_is_req msg = true /\ Serial' hst' (Some idx)
         end
       end.
 
-    Definition serial (hst: list IMsg) := serial' hst None.
+    Definition Serial (hst: list IMsg) := Serial' hst None.
 
     Definition subHistory (i: IdxT) (hst: list IMsg) :=
       filter (fun e => if eq_nat_dec i (fst e) then true else false) hst.
@@ -172,12 +192,74 @@ Section Language.
       forall i, subHistory i hst1 = subHistory i hst2.
 
     Definition Serializable (hst: list IMsg) :=
-      exists str, serial str /\ Equivalent hst str.
+      exists shst, Serial shst /\ Equivalent (complete hst) shst.
 
     Definition SerialObjects (obs: Objects) :=
       forall hst, HistoryOf obs hst -> Serializable hst.
 
   End Semantics.
+
+  Section Facts.
+
+    Lemma equivalent_refl: forall hst, Equivalent hst hst.
+    Proof.
+      unfold Equivalent; intros; reflexivity.
+    Qed.
+    Hint Immediate equivalent_refl.
+
+    Lemma equivalent_app:
+      forall hst1 hst1' hst2 hst2',
+        Equivalent hst1 hst1' -> Equivalent hst2 hst2' ->
+        Equivalent (hst1 ++ hst2) (hst1' ++ hst2').
+    Proof.
+    Admitted.
+
+    Lemma complete_serial: forall hst, Serial hst -> Serial (complete hst).
+    Proof.
+    Admitted.
+    Hint Immediate complete_serial.
+
+    Lemma complete_serial_app:
+      forall hst1,
+        Complete hst1 ->
+        forall hst2, Serial hst2 -> Serial (hst1 ++ hst2).
+    Proof.
+    Admitted.
+    Hint Immediate complete_serial_app.
+
+    Lemma complete_complete_app:
+      forall hst1,
+        Complete hst1 ->
+        forall hst2, complete (hst1 ++ hst2) = complete hst1 ++ complete hst2.
+    Proof.
+    Admitted.
+
+    Lemma complete_equivalent:
+      forall hst, Complete hst -> Equivalent (complete hst) hst.
+    Proof.
+    Admitted.
+    Hint Immediate complete_equivalent.
+      
+    Lemma serial_serializable: forall hst, Serial hst -> Serializable hst.
+    Proof.
+      intros; exists (complete hst); split; eauto.
+    Qed.
+    Hint Immediate serial_serializable.
+
+    Lemma complete_serializable_app:
+      forall hst1,
+        Complete hst1 ->
+        forall hst2, Serializable hst2 -> Serializable (hst1 ++ hst2).
+    Proof.
+      unfold Serializable; intros.
+      destruct H0 as [shst2 [? ?]].
+      exists (hst1 ++ shst2); split; auto.
+
+      rewrite complete_complete_app by assumption.
+      apply equivalent_app; auto.
+    Qed.
+
+  End Facts.
 
 End Language.
 
