src/Prototype/Correctness.v
@@ -1,0 +1,7 @@
+Require Import List String Peano_dec.
+Require Import Language SingleValue.
+
+Theorem impl_serial: SerialObjects svm_is_req impl.
+Proof.
+  unfold SerialObjects, HistoryOf, Serializable; intros.
+Admitted.
